module Cwf.UniType.Lemmata where

open import Base.Core
open import Base.FinFun
open import Cwf.UniType.Definition
open import Cwf.UniType.Relation

open import Agda.Builtin.Bool
open import Agda.Builtin.Equality
open import Agda.Builtin.Size

getCff : âˆ€ {i} â†’ {ğ‘“ : FinFun (Nbh {i}) (Nbh {i})} â†’
         {x y xâ€² yâ€² : Nbh {i}} â†’ ConFinFun ğ‘“ â†’
         (x , y) âˆˆ ğ‘“ â†’ (xâ€² , yâ€²) âˆˆ ğ‘“ â†’
         Con x xâ€² â†’ Con y yâ€²
getCff (cff p) = p

cffSym : âˆ€ {i} â†’ {ğ‘“ ğ‘” : FinFun (Nbh {i}) (Nbh {i})} â†’
         ConFinFun (ğ‘“ âˆª ğ‘”) â†’ ConFinFun (ğ‘” âˆª ğ‘“)
cffSym {ğ‘“ = ğ‘“} (cff p)
  = cff Î» xyâˆˆğ‘“âˆªğ‘” xâ€²yâ€²âˆˆğ‘“âˆªğ‘” â†’ p (âˆª-lemmaâ‚ˆ {ğ‘“â€² = ğ‘“} xyâˆˆğ‘“âˆªğ‘”)
    (âˆª-lemmaâ‚ˆ {ğ‘“â€² = ğ‘“} xâ€²yâ€²âˆˆğ‘“âˆªğ‘”)

conSym : âˆ€ {i} â†’ {x y : Nbh {i}} â†’ Con x y â†’ Con y x
conSym con-âŠ¥â‚ = con-âŠ¥â‚‚
conSym con-âŠ¥â‚‚ = con-âŠ¥â‚
conSym con-refl-0 = con-refl-0
conSym (con-s consxsy) = con-s (conSym consxsy)
conSym con-refl-â„• = con-refl-â„•
conSym con-refl-ğ’° = con-refl-ğ’°
conSym (con-Î  {ğ‘“ = ğ‘“} conxy cffğ‘“âˆªğ‘”)
  = con-Î  (conSym conxy) (cffSym {ğ‘“ = ğ‘“} cffğ‘“âˆªğ‘”)
conSym (con-Î» {ğ‘“ = ğ‘“} cffâˆª) = con-Î» (cffSym {ğ‘“ = ğ‘“} cffâˆª)

liftÎ»-proof : âˆ€ {i} â†’ {ğ‘“ ğ‘“â€² : FinFun (Nbh {i}) (Nbh {i})} â†’
              âˆ€ {conğ‘“ conğ‘“â€² x y} â†’ ğ‘“ âŠ† ğ‘“â€² â†’
              Î»-proof ğ‘“ conğ‘“ x y â†’ Î»-proof ğ‘“â€² conğ‘“â€² x y
liftÎ»-proof ğ‘“âŠ†ğ‘“â€²
  record
      { sub = sub
      ; subâŠ†ğ‘“ = subâŠ†ğ‘“
      ; preablesub = preablesub
      ; postablesub = postablesub
      ; yâŠ‘post = yâŠ‘post
      ; preâŠ‘x = preâŠ‘x
      }
  = record
      { sub = sub
      ; subâŠ†ğ‘“ = âŠ†-trans subâŠ†ğ‘“ ğ‘“âŠ†ğ‘“â€²
      ; preablesub = preablesub
      ; postablesub = postablesub
      ; yâŠ‘post = yâŠ‘post
      ; preâŠ‘x = preâŠ‘x
      }

shrinkÎ»-proof : âˆ€ {i} â†’ {ğ‘“ ğ‘“â€² ğ‘“â€³ : FinFun (Nbh {i}) (Nbh {i})} â†’
                âˆ€ {conğ‘“â€² conğ‘“â€³} â†’ ğ‘“ âŠ† ğ‘“â€² â†’
                Î»áµ¤ ğ‘“â€² conğ‘“â€² âŠ‘áµ¤ Î»áµ¤ ğ‘“â€³ conğ‘“â€³ â†’
                âˆ€ {x y} â†’ (x , y) âˆˆ ğ‘“ â†’
                Î»-proof ğ‘“â€³ conğ‘“â€³ x y
shrinkÎ»-proof ğ‘“âŠ†ğ‘“â€² (âŠ‘áµ¤-Î» p) xyâˆˆğ‘“ = p (ğ‘“âŠ†ğ‘“â€² xyâˆˆğ‘“)
